Add theorems 3.5.7 and 3.5.8

untyped_arithmetic_expressions.thy
@@ -7,6 +7,17 @@ datatype B_term
   | BFalse
   | BIf B_term B_term B_term
 
+inductive is_value :: "B_term \<Rightarrow> bool" where
+  "is_value BTrue" |
+  "is_value BFalse"
+
+thm is_value.induct
+thm is_value.intros
+thm is_value.cases
+thm is_value.simps
+
+inductive_cases is_value_BIfD: "is_value (BIf t1 t2 t3)"
+
 inductive eval_once :: "B_term \<Rightarrow> B_term \<Rightarrow> bool" where
   e_if_true: "eval_once (BIf BTrue t2 t3) t2" |
   e_if_false: "eval_once (BIf BFalse t2 t3) t3" |
@@ -16,6 +27,12 @@ thm eval_once.induct
 thm eval_once.intros
 thm eval_once.cases
 thm eval_once.simps
+
+inductive_cases eval_once_BTrueD: "eval_once BTrue t"
+inductive_cases eval_once_BFalseD: "eval_once BFalse t"
+
+inductive is_normal_form :: "B_term \<Rightarrow> bool" where
+  "\<forall>t'. \<not> eval_once t t' \<Longrightarrow> is_normal_form t"
 
 lemma
   assumes
@@ -32,9 +49,6 @@ proof -
     by (rule e_if)
 qed
 
-inductive_cases eval_once_BTrueD: "eval_once BTrue t"
-inductive_cases eval_once_BFalseD: "eval_once BFalse t"
-
 lemma not_eval_once_BTrue: "\<not> eval_once BTrue t"
   by (blast dest: eval_once_BTrueD)
 
@@ -47,13 +61,11 @@ lemma
   shows "eval_once t t' \<Longrightarrow> eval_once t t'' \<Longrightarrow> t' = t''"
 proof (induction t t' arbitrary: t'' rule: eval_once.induct)
   case (e_if_true t1 t2)
-  thus ?case
-    by (auto dest: eval_once_BTrueD elim: eval_once.cases)
+  thus ?case by (auto dest: eval_once_BTrueD elim: eval_once.cases)
     (* by (auto simp: not_eval_once_BTrue elim: eval_once.cases) *)
 next
   case (e_if_false t1 t2)
-  thus ?case
-    by (auto simp: not_eval_once_BTrue elim: eval_once.cases)
+  thus ?case by (auto simp: not_eval_once_BTrue elim: eval_once.cases)
 next
   case (e_if t1 t1' t2 t3)
   show ?case
@@ -65,6 +77,25 @@ next
     apply (rename_tac t1'')
     apply (erule e_if.IH)
     done *)
+qed
+
+theorem
+  fixes t :: B_term
+  shows "is_value t \<Longrightarrow> is_normal_form t"
+using eval_once_BFalseD eval_once_BTrueD is_normal_form.intros is_value.simps by fastforce
+
+theorem
+  fixes t :: B_term
+  shows "is_normal_form t \<Longrightarrow> is_value t"
+proof (rule ccontr, induction t rule: B_term.induct)
+    case BTrue
+    thus ?case by (simp add: is_value.intros(1))
+  next
+    case BFalse
+    thus ?case by (simp add: is_value.intros(2))
+  next
+    case (BIf t1 t2 t3)
+    thus ?case by (metis e_if e_if_false e_if_true is_normal_form.cases is_normal_form.intros is_value.cases)
 qed
 
 end
